src/program_proof/disk_lib.v
@@ -19,12 +19,14 @@ Proof.
     auto.
 Qed.
 
-(* TODO: this should probably also have a fraction *)
 Definition is_block (s:Slice.t) (q: Qp) (b:Block) :=
   is_slice_small s byteT q (Block_to_vals b).
 
 Definition is_block_full (s:Slice.t) (b:Block) :=
   is_slice s byteT 1 (Block_to_vals b).
+
+Global Instance is_block_timeless s q b :
+  Timeless (is_block s q b) := _.
 
 Definition list_to_block (l: list u8) : Block :=
   match decide (length l = Z.to_nat 4096) with
